Fix allocator spec to match Coq proof

dafny_go/jrnl/alloc.go
@@ -7,11 +7,12 @@ type Allocator struct {
 }
 
 func NewAllocator(max uint64) *Allocator {
-	if max == 0 {
-		panic("invalid max, must be at least 0")
+	if !(0 < max && max%8 == 0) {
+		panic("invalid max, must be at least 0 and divisible by 8")
 	}
 	num_bytes := max / 8
 	a := alloc.MkAlloc(make([]byte, num_bytes))
+	a.MarkUsed(0)
 	return &Allocator{alloc: *a}
 }
 
@@ -24,9 +25,5 @@ func (a *Allocator) Alloc() uint64 {
 }
 
 func (a *Allocator) Free(x uint64) {
-	// avoid panic in alloc implementation
-	if x == 0 {
-		return
-	}
 	a.alloc.FreeNum(x)
 }
