dafny_go/jrnl/alloc_test.go
@@ -12,8 +12,7 @@ func getArbitrary(m map[uint64]bool) uint64 {
 func TestAllocator(t *testing.T) {
 	// the allocator has no preconditions so we just attempt to exercise it a bit
 	used := make(map[uint64]bool)
-	a := NewAllocator(100)
-	a.MarkUsed(0)
+	a := NewAllocator(128)
 
 	for i := 0; i < 20; i++ {
 		x := a.Alloc()
